Iris/Iris/HeapLang/Lib/SpinLock.lean
@@ -1,0 +1,142 @@
+module
+
+public import Iris.HeapLang.Lib.Lock
+public import Iris.Instances.Lib.Token
+public import Iris.Instances.Lib.Invariants
+public import Iris.Std.Namespaces
+public import Iris.HeapLang.PrimitiveLaws
+
+namespace Iris.HeapLang
+
+open BI Iris
+
+@[expose] public section
+
+def spinlock_newlock : Val := hl_val(λ _, ref(#false))
+def spinlock_try_acquire : Val := hl_val(λ l, cas(l, #false, #true))
+def spinlock_acquire : Val :=
+  hl_val(rec acquire l := if {spinlock_try_acquire} l then #() else acquire l)
+def spinlock_release : Val := hl_val(λ l, l ← #false)
+
+abbrev SpinLockG (GF : BundledGFunctors) := TokenG GF
+
+def spinlockN : Namespace := ndot nroot "spinlock"
+
+section SpinLockPredicates
+
+variable [HeapLangGS hlc GF] [SpinLockG GF]
+
+def locked (γ : GName) : IProp GF := token γ
+
+def lock_inv (γ : GName) (l : Loc) (R : IProp GF) : IProp GF :=
+  iprop(∃ b : Bool, (l ↦ Option.some hl_val(#b)) ∗ (if b then True else token γ ∗ R))
+
+def is_lock (γ : GName) (lk : Val) (R : IProp GF) : IProp GF :=
+  iprop(∃ l : Loc, ⌜lk = Val.lit (.loc l)⌝ ∧ inv spinlockN (lock_inv γ l R))
+
+instance is_lock_persistent (γ : GName) (lk : Val) (R : IProp GF) :
+    Persistent (is_lock γ lk R) := by
+  unfold is_lock; infer_instance
+
+instance locked_timeless (γ : GName) : Timeless (locked (GF := GF) γ) := by
+  unfold locked; infer_instance
+
+theorem locked_exclusive (γ : GName) :
+    (locked γ ∗ locked γ) ⊢@{IProp GF} False :=
+  token_exclusive γ
+
+theorem is_lock_iff (γ : GName) (lk : Val) (R₁ R₂ : IProp GF) :
+    is_lock γ lk R₁ ⊢ (▷ □ (R₁ ∗-∗ R₂)) -∗ is_lock γ lk R₂ := by
+  unfold is_lock lock_inv
+  iintro ⟨%l, %H1, #H2⟩ Heq
+  iexists l
+  isplit; itrivial
+  iapply inv_iff $$ H2
+  inext; icases Heq with #Heq; imodintro
+  isplit
+  · iintro ⟨%b, H1, H3⟩
+    iexists b; iframe H1
+    split; itrivial
+    icases H3 with ⟨$, H3⟩
+    iapply Heq $$ H3
+  · iintro ⟨%b, H1, H3⟩
+    iexists b; iframe H1
+    split; itrivial
+    icases H3 with ⟨$, H3⟩
+    iapply Heq $$ H3
+
+end SpinLockPredicates
+
+section SpinLockSpecs
+
+variable {GF : BundledGFunctors} [HeapLangGS hlc GF] [SpinLockG GF]
+
+theorem spinlock_newlock_spec :
+  ⊢ □ ∀ (Φ : Val → IProp GF),
+    (∀ (v : Val) (γ : GName), (∀ R E, R ={E}=∗ is_lock γ v R) -∗ Φ v)
+    -∗ WP hl({spinlock_newlock} #()) {{ Φ }} := by
+  unfold spinlock_newlock
+  imodintro
+  iintro %Φ Hcont
+  iapply wp_rec; simp only [Exp.subst]
+  inext
+  imod token_alloc with ⟨%γ, Hγ⟩
+  iapply wp_wand (Φ := fun v => iprop(∃ l', ⌜v = hl_val(#(BaseLit.loc l'))⌝ ∗ l' ↦ some hl_val(#false)))
+  · iapply wp_alloc
+  iintro %v ⟨%l, %Heq, Hpt⟩
+  iapply Hcont $$ %v %γ
+  iintro %R %E HR
+  imod inv_alloc spinlockN E iprop(∃ b, (l ↦ some hl_val(#(BaseLit.bool b))) ∗ if b = true then True else token γ ∗ R) $$ [Hpt HR Hγ]
+  · iexists false
+    simp only [Bool.false_eq_true, ↓reduceIte]
+    inext; iframe
+  · subst Heq
+    imodintro
+    unfold is_lock
+    iexists l
+    isplit; itrivial
+    unfold lock_inv
+    iframe
+
+theorem spinlock_try_acquire_spec (γ : GName) (lk : Val) (R : IProp GF) :
+    ⊢ □ ∀ (Φ : Val → IProp GF),
+    is_lock γ lk R
+    -∗ (((locked γ ∗ R) -∗ Φ (.lit (.bool true))) ∧
+     (True -∗ Φ (.lit (.bool false))))
+    -∗ WP hl({spinlock_try_acquire} {lk}) {{ Φ }} := by
+  sorry
+
+theorem spinlock_acquire_spec (γ : GName) (lk : Val) (R : IProp GF) :
+  ⊢ □ ∀ (Φ : Val → IProp GF),
+    is_lock γ lk R
+    -∗ ((locked γ ∗ R) -∗ Φ (.lit .unit))
+    -∗ WP hl({spinlock_acquire} {lk}) {{ Φ }} := by
+  sorry
+
+theorem spinlock_release_spec (γ : GName) (lk : Val) (R : IProp GF) :
+  ⊢ □ ∀ (Φ : Val → IProp GF),
+    (is_lock γ lk R ∗ locked γ ∗ R)
+    -∗ (True -∗ Φ (.lit .unit))
+    -∗ WP hl({spinlock_release} {lk}) {{ Φ }} := by
+  sorry
+
+end SpinLockSpecs
+
+@[implicit_reducible]
+def spinLock [HeapLangGS hlc GF] : lock GF where
+  newlock := spinlock_newlock
+  acquire := spinlock_acquire
+  release := spinlock_release
+  lockG   := SpinLockG
+  name := GName
+  is_lock _ γ lk R  := is_lock γ lk R
+  locked _ γ := locked γ
+  is_lock_persistent γ lk R := is_lock_persistent γ lk R
+  is_lock_iff γ lk R₁ R₂ := is_lock_iff γ lk R₁ R₂
+  locked_timeless γ := locked_timeless γ
+  locked_exclusive γ := locked_exclusive γ
+  newlock_spec_delay_init Φ := spinlock_newlock_spec Φ
+  acquire_spec γ lk R Φ := spinlock_acquire_spec γ lk R Φ
+  release_spec γ lk R Φ := spinlock_release_spec γ lk R Φ
+
+end
